Makefile
@@ -15,6 +15,7 @@ DEP_FLAG = $(DEP_DEMO)
 lib_FILES = \
   Coqlib.v Ensembles_ext.v Relation_ext.v Equivalence_ext.v List_Func_ext.v \
   Bijection.v Countable.v NatChoice.v StrongInduction.v \
+  SublistT.v \
   Stream/SigStream.v Stream/StreamFunctions.v Stream/StreamSplit.v 
 
 GeneralLogic_ShallowEmbedded_FILES = \
